changes to the journal -- journal.i.dfy times out

Splinter/JournalInterp.i.dfy
@@ -82,21 +82,11 @@ module JournalInterpMod {
 //    CrashTolerantMapSpecMod.Variables(versions, 0)
 //  }
 
-  function ReadAt(cus: seq<CU>, i: nat) : AU
-    requires i<|cus|
-  {
-    cus[i].au
-  }
-
   // TODO(jonh): Try porting this from recursive style to Travis' suggested
   // repr-state style (see ReprsAsSets.i.dfy).
-  function IReads(v: Variables, cache:CacheIfc.Variables, sb: CoreSuperblock) : seq<AU>
+  function IReads(v: Variables, cache:CacheIfc.Variables, sb: CoreSuperblock) : seq<CU>
   {
-    var cus := ChainFrom(cache.dv, sb).readCUs;
-    // wanted to write:
-    // seq(|cus|, i requires 0<=i<|cus| => cus[i].au)
-    // but Dafny bug, so:
-    seq(|cus|, i requires 0<=i<|cus| => ReadAt(cus, i))
+    ChainFrom(cache.dv, sb).readCUs
   }
 
   predicate SequenceSubset<T>(a:seq<T>, b:seq<T>)
@@ -104,10 +94,10 @@ module JournalInterpMod {
     forall i | 0<=i<|a| :: a[i] in b
   }
 
-  lemma DiskViewsEquivalentAfterRemove(cache0: CacheIfc.Variables, cache1: CacheIfc.Variables, aus: seq<AU>, removedCU: CU, ausr: seq<AU>)
-    requires DiskViewsEquivalentForSet(cache0.dv, cache1.dv, aus)
-    requires SequenceSubset(ausr, aus)
-    ensures DiskViewsEquivalentForSet(MapRemove1(cache0.dv, removedCU), MapRemove1(cache1.dv, removedCU), ausr)
+  lemma DiskViewsEquivalentAfterRemove(cache0: CacheIfc.Variables, cache1: CacheIfc.Variables, cus: seq<CU>, removedCU: CU, cusr: seq<CU>)
+    requires DiskViewsEquivalentForSet(cache0.dv, cache1.dv, cus)
+    requires SequenceSubset(cusr, cus)
+    ensures DiskViewsEquivalentForSet(MapRemove1(cache0.dv, removedCU), MapRemove1(cache1.dv, removedCU), cusr)
   {
   }
 
@@ -118,7 +108,9 @@ module JournalInterpMod {
     decreases |cache0.dv|
   {
     if sb.freshestCU.Some? {
-      assert IReads(v, cache0, sb)[0] == sb.freshestCU.value.au; // trigger
+      assert sb.freshestCU.value in IReads(v, cache1, sb); // trigger
+      assert sb.freshestCU.value in IReads(v, cache0, sb); // trigger
+      assert IReads(v, cache0, sb)[0] == sb.freshestCU.value; // trigger
       if sb.freshestCU.value in cache0.dv {
         var firstRec := parse(cache0.dv[sb.freshestCU.value]);
         if firstRec.Some? { // Recurse to follow chain
@@ -130,15 +122,23 @@ module JournalInterpMod {
             var cache1r := CacheIfc.Variables(MapRemove1(cache1.dv, sb.freshestCU.value));
             var priorCU := firstRec.value.priorCU;
             var priorSB := firstRec.value.priorSB(sb);
-            var aus := IReads(v, cache0, sb);
-            var ausr := if priorCU.Some?
+            var cus := IReads(v, cache0, sb);
+            var cusr := if priorCU.Some?
               then IReads(v, cache0r, priorSB)
               else [];
 
-            forall i | 0<=i<|ausr| ensures ausr[i] in aus {
-              assert aus[i+1] == ausr[i]; // witness to SequenceSubset(ausr, aus)
+            assert cache0r.dv == MapRemove1(cache0.dv, sb.freshestCU.value);
+            assert firstRec.value.priorSB(sb) == priorSB;
+            calc {
+              ChainFrom(cache0.dv, sb).readCUs;
+              [sb.freshestCU.value] + ChainFrom(cache0r.dv, priorSB).readCUs;
             }
-            DiskViewsEquivalentAfterRemove(cache0, cache1, aus, sb.freshestCU.value, ausr);
+            assert ChainFrom(cache0.dv, sb).readCUs == [sb.freshestCU.value] + ChainFrom(cache0r.dv, priorSB).readCUs;
+
+            forall i | 0<=i<|cusr| ensures cusr[i] in cus {
+              assert cus[i+1] == cusr[i]; // witness to SequenceSubset(ausr, aus)
+            }
+            DiskViewsEquivalentAfterRemove(cache0, cache1, cus, sb.freshestCU.value, cusr);
             FrameOneChain(v, cache0r, cache1r, priorSB);
           }
         }
